theories/iris/examples/effects/coroutines_module.v
@@ -1,0 +1,162 @@
+
+From mathcomp Require Import ssreflect eqtype seq ssrbool.
+From iris.program_logic Require Import language.
+From iris.proofmode Require Import base tactics classes.
+From iris.base_logic Require Export gen_heap ghost_map proph_map.
+From iris.base_logic.lib Require Export fancy_updates.
+From iris.bi Require Export weakestpre.
+From Wasm.iris.rules Require Export iris_rules iris_example_helper.
+From Wasm.iris.host Require Export iris_host.
+From Wasm.iris.examples.effects Require Import coroutines_implementation_code.
+
+
+Set Bullet Behavior "Strict Subproofs".
+Set Implicit Arguments.
+Unset Strict Implicit.
+Unset Printing Implicit Defensive.
+
+
+Section CoroutinesModule.
+  Context `{!wasmG Σ, !hvisG Σ, !hmsG Σ, !hasG Σ}.
+
+  Definition coroutines_module :=
+    {|
+      mod_types := [ emptyt ; par_type ];
+      mod_funcs :=
+      [ {|
+          modfunc_type := Mk_typeidx 0 ;
+          modfunc_locals := [] ;
+          modfunc_body := yield
+        |};
+        {|
+          modfunc_type := Mk_typeidx 1 ;
+          modfunc_locals := par_locs ;
+          modfunc_body := par
+        |}
+      ] ;
+      mod_tables := [];
+      mod_mems := [] ;
+      mod_globals := [];
+      mod_elem := [] ;
+      mod_data := [] ;
+      mod_start := None; 
+      mod_imports := [];
+      mod_exports := [
+        {| modexp_name := String.list_byte_of_string "yield function" ;
+          modexp_desc :=
+            MED_func (Mk_funcidx 0) |} ;
+        {| modexp_name := String.list_byte_of_string "par function" ;
+          modexp_desc :=
+            MED_func (Mk_funcidx 1) |}
+      ];
+      mod_tags := [emptyt]
+    |}.
+
+  Definition expts := [ET_func emptyt ; ET_func par_type].
+
+  Lemma coroutines_module_typing :
+    module_typing coroutines_module [] expts.
+  Proof.
+    unfold module_typing.
+    exists [emptyt; par_type], []. simpl.
+    repeat split;eauto.
+    - rewrite ! Forall2_cons. repeat split;auto; cbn;auto.
+      + apply yield_typing. 
+      + apply par_typing.
+    - constructor => //. constructor => //. 
+  Qed.
+
+  Definition coroutines_module_instantiate yield_exp_addr par_exp_addr mod_addr:=
+    [ ID_instantiate [ yield_exp_addr ; par_exp_addr ] mod_addr [] ].
+
+  Notation "{{{{ P }}}} es {{{{ v , Q }}}}" :=
+    (□ ∀ Φ, P -∗ (∀ v, Q -∗ Φ v) -∗ WP (es : host_expr) @ NotStuck ; ⊤ {{ v, Φ v }})%I (at level 50).
+
+  Lemma instantiate_coroutines yield_exp_addr par_exp_addr mod_addr: 
+    
+    ⊢ {{{{ 
+              mod_addr ↪[mods] coroutines_module ∗
+                (∃ exp1, yield_exp_addr ↪[vis] exp1) ∗
+                (∃ exp2, par_exp_addr ↪[vis] exp2)
+      }}}}
+      ((coroutines_module_instantiate yield_exp_addr par_exp_addr mod_addr,
+         [], empty_frame) : host_expr) 
+        {{{{  x,  ⌜x = (immHV [], empty_frame)⌝ ∗
+                          mod_addr ↪[mods] coroutines_module ∗
+                          ∃ addr_yield addr_par name_yield name_par cl_yield cl_par,
+                            yield_exp_addr ↪[vis] {| modexp_name := name_yield;
+                                                    modexp_desc := MED_func (Mk_funcidx addr_yield) |} ∗
+                              par_exp_addr ↪[vis] {| modexp_name := name_par;
+                                                    modexp_desc := MED_func (Mk_funcidx addr_par) |} ∗
+                              N.of_nat addr_yield ↦[wf] cl_yield ∗
+                              N.of_nat addr_par ↦[wf] cl_par ∗
+                              yield_par_spec addr_yield addr_par cl_yield cl_par
+                         
+        }}}} .
+  Proof.
+    iIntros "!>" (Φ) "(Hmod & Hvis1 & Hvis2) HΦ".
+    iApply (weakestpre.wp_wand _ _ (_ : host_expr) with "[- HΦ]").
+    iApply (instantiation_spec_operational_no_start with "[$Hmod Hvis1 Hvis2]") => //.
+    - apply coroutines_module_typing. 
+    - unfold module_restrictions. cbn. repeat split;exists [];auto. 
+    - iFrame. 
+      iSplitR.
+      instantiate (1:=[]).
+      unfold import_resources_host.
+      simpl. done.
+      repeat instantiate (1:=∅).
+      iSplitR; last by simpl.
+      rewrite /instantiation_resources_pre_wasm /import_resources_wasm_typecheck
+        /import_func_wasm_check /import_tab_wasm_check /import_glob_wasm_check
+        /import_mem_wasm_check /import_tag_wasm_check.
+      repeat iSplit.
+      all: try by iApply big_sepM_empty.
+      all: iPureIntro.
+      all: try done.
+      all: try constructor.
+    - iIntros (v) "(-> & H)".
+      iApply "HΦ".
+      iSplit; first done.
+      unfold instantiation_resources_post.
+      iDestruct "H" as "(Hmod & Himports & %inst & Hresources & Hexports)".
+      iDestruct "Hexports" as "([%name1 Hexp1] & [%name2 Hexp2] & _)".
+      simpl.
+      iFrame.
+      unfold instantiation_resources_post_wasm.
+      iDestruct "Hresources" as (g_inits tab_allocs mem_allocs glob_allocs tag_allocs wts' wms') "(Himport_typecheck & %Hprefixes & -> & -> & %Helembound & -> & -> & %Hdatabound & %Hinit & -> & -> & Hresources)".
+      unfold module_inst_resources_wasm.
+      iDestruct "Hresources" as "(Hfuncs & Htabs & Hmems & Hglobs & Htags)".
+      rewrite /get_import_func_count /get_import_table_count /get_import_mem_count
+        /get_import_global_count /get_import_tag_count /= /drop
+        /module_inst_resources_func /module_inst_resources_tab /module_inst_resources_mem
+        /module_inst_resources_glob /module_inst_resources_tag
+      .
+      destruct inst.
+      simpl.
+      destruct inst_globs; last done.
+      destruct inst_memory; last done.
+      destruct inst_tab; last done.
+      iClear "Htabs Hmems Hglobs".
+      destruct inst_funcs; first done.
+      iDestruct "Hfuncs" as "[Hyield Hfuncs]".
+      destruct inst_funcs; first done.
+      iDestruct "Hfuncs" as "[Hpar Hfuncs]".
+      destruct inst_funcs; last done.
+      iClear "Hfuncs".
+      destruct inst_tags; first done.
+      iDestruct "Htags" as "[#Htag Htags]".
+      destruct inst_tags; last done.
+      iClear "Htags".
+      simpl.
+      simpl in Hprefixes.
+      destruct Hprefixes as [-> Hprefixes].
+
+      iFrame.
+      iApply yield_par_spec_proof.
+      done.
+      done.
+      iFrame "Htag".
+  Qed. 
+    
+    
+End CoroutinesModule.
